need an assumption of non-duplicate message delivery. What is the simplest way to axiomatize that. Added a comment explained why we didn't need it in the train case.
Fixed an issue in the statement of the proof by defining an operator
on lists that substitutes the head with something

StdlibMisc.v
@@ -104,6 +104,9 @@ Coercion assert : bool >-> Sortclass.
 
 Inductive void: Set :=.
 
+(** Using typeclasses, this can be made to work for other types of products,
+    e.g. propositional conjunctions *)
+
 Notation π₁ := fst.
 Notation π₂ := snd.
 
@@ -113,3 +116,8 @@ Definition subList {T : Type} (start length : nat) (l : list T) : list T :=
 Definition isPrefixOf {T : Type} (lp l : list T) : Prop :=
   firstn  (length lp) l =lp.
 
+Definition substHead {A : Type} (l : list A) (h' : A) :=
+match l with
+| nil => nil
+| h::tl => h'::tl
+end.
